src/tactic/field/norm.lean
@@ -10,9 +10,9 @@ end list
 
 namespace field
 
-inductive alt {γ} [const_space γ] : bool → Type
-| sform : list (@nterm γ _) → @sterm γ _ → alt tt
-| pform : list (@nterm γ _) → @pterm γ _ → alt ff
+inductive alt (γ) [const_space γ] : bool → Type
+| sform : list (nterm γ) → sterm γ → alt tt
+| pform : list (nterm γ) → pterm γ → alt ff
 
 namespace alt
 open nterm
@@ -21,40 +21,40 @@ variables {α : Type} [discrete_field α]
 variables {γ : Type} [const_space γ]
 variables [morph γ α] {ρ : dict α}
 
-def of_const (a : γ) : Π {b}, @alt γ _ b
+def of_const (a : γ) : Π {b}, alt γ b
 | tt := sform [] (sterm.of_const a)
 | ff := pform [] (pterm.of_const a)
 
-def singleton (x : @nterm γ _) : Π {b}, @alt γ _ b
+def singleton (x : nterm γ) : Π {b}, alt γ b
 | tt := sform ∅ (sterm.singleton x)
 | ff := pform ∅ (pterm.singleton x)
 
-def to_nterm : @alt γ _ tt → @nterm γ _
+def to_nterm : alt γ tt → nterm γ
 | (sform _ S) := S.to_nterm
 
-def to_sterm : @alt γ _ tt → @sterm γ _
+def to_sterm : alt γ tt → sterm γ
 | (sform _ S) := S
 
-def to_pterm : @alt γ _ ff → @pterm γ _
+def to_pterm : alt γ ff → pterm γ
 | (pform _ P) := P
 
-def hyps : Π {b}, @alt γ _ b → list (@nterm γ _)
+def hyps : Π {b}, alt γ b → list (nterm γ)
 | ._ (sform ts _) := ts
 | ._ (pform ts _) := ts
 
-def eval (ρ : dict α) : Π {b}, @alt γ _ b → α
+def eval (ρ : dict α) : Π {b}, alt γ b → α
 | ._ (sform _ S) := sterm.eval ρ S
 | ._ (pform _ P) := pterm.eval ρ P
 
-def to_sform : Π {b}, @alt γ _ b → @alt γ _ tt
+def to_sform : Π {b}, alt γ b → alt γ tt
 | ._ (sform ts S) := sform ts S
 | ._ (pform ts P) := sform (ts ∪ P.reduce_hyps) (sterm.of_nterm P.reduce.to_nterm)
 
-def to_pform : Π {b}, @alt γ _ b → @alt γ _ ff
+def to_pform : Π {b}, alt γ b → alt γ ff
 | ._ (sform ts S) := pform ts (pterm.of_nterm S.to_nterm)
 | ._ (pform ts P) := pform ts P
 
-def hyps_to_sform {a} {x : @alt γ _ a} :
+def hyps_to_sform {a} {x : alt γ a} :
   x.hyps ⊆ x.to_sform.hyps :=
 begin
   cases x,
@@ -62,20 +62,20 @@ begin
   { unfold to_sform, unfold hyps, exact list.subset_union_left }
 end
 
-def hyps_to_pform {a} {x : @alt γ _ a} :
+def hyps_to_pform {a} {x : alt γ a} :
   x.hyps = x.to_pform.hyps :=
 by cases x; simp [hyps, to_pform]
 
-theorem eval_def {x : @alt γ _ tt} :
+theorem eval_def {x : alt γ tt} :
   eval ρ x = nterm.eval ρ x.to_nterm :=
 by {cases x, simp [eval, to_nterm, sterm.eval_to_nterm]}
 
 theorem eval_of_const {b} {c : γ} :
-  eval ρ (of_const c : @alt γ _ b) = (c : α) :=
+  eval ρ (of_const c : alt γ b) = (c : α) :=
 by cases b; simp [of_const, eval, pterm.eval_of_const, sterm.eval_of_const]
 
-theorem eval_singleton {b} {x : @nterm γ _} :
-  eval ρ (singleton x : @alt γ _ b) = nterm.eval ρ x :=
+theorem eval_singleton {b} {x : nterm γ} :
+  eval ρ (singleton x : alt γ b) = nterm.eval ρ x :=
 begin
   cases b,
   { unfold singleton, unfold eval,
@@ -84,7 +84,7 @@ begin
     rw ← sterm.eval_singleton }
 end
 
-theorem eval_to_sform {b} {x : @alt γ _ b} :
+theorem eval_to_sform {b} {x : alt γ b} :
   nonzero ρ x.to_sform.hyps →
   eval ρ x.to_sform = eval ρ x :=
 begin
@@ -99,7 +99,7 @@ begin
     exact ht }
 end
 
-theorem eval_to_pform {b} {x : @alt γ _ b} :
+theorem eval_to_pform {b} {x : alt γ b} :
   eval ρ x.to_pform = eval ρ x :=
 begin
   cases x,
@@ -108,13 +108,13 @@ begin
   { refl }
 end
 
-theorem eval_to_sterm {x : @alt γ _ tt} :
+theorem eval_to_sterm {x : alt γ tt} :
   sterm.eval ρ x.to_sterm = eval ρ x :=
 begin
   cases x, unfold to_sterm, unfold eval
 end
 
-theorem eval_to_pterm {x : @alt γ _ ff} :
+theorem eval_to_pterm {x : alt γ ff} :
   eval ρ x = pterm.eval ρ x.to_pterm :=
 begin
   cases x, unfold to_pterm, unfold eval
@@ -124,42 +124,42 @@ end
 --more cases to avoid switching form too often
 --when applying operators
 
-def add_sform (x y : @alt γ _ tt) : @alt γ _ tt :=
+def add_sform (x y : alt γ tt) : alt γ tt :=
 sform (x.hyps ∪ y.hyps) (x.to_sterm + y.to_sterm)
 
-def mul_pform (x y : @alt γ _ ff) : @alt γ _ ff :=
+def mul_pform (x y : alt γ ff) : alt γ ff :=
 pform (x.hyps ∪ y.hyps) (x.to_pterm * y.to_pterm)
 
-def pow_pform (x : @alt γ _ ff) (n : znum) : @alt γ _ ff :=
+def pow_pform (x : alt γ ff) (n : znum) : alt γ ff :=
 if n = 0 then singleton (1 : γ)
 else pform x.hyps (x.to_pterm ^ n)
 
-instance : has_add (@alt γ _ tt) := ⟨add_sform⟩
-instance : has_mul (@alt γ _ ff) := ⟨mul_pform⟩
-instance : has_pow (@alt γ _ ff) znum := ⟨pow_pform⟩
+instance : has_add (alt γ tt) := ⟨add_sform⟩
+instance : has_mul (alt γ ff) := ⟨mul_pform⟩
+instance : has_pow (alt γ ff) znum := ⟨pow_pform⟩
 
-def add {a b} (x : @alt γ _ a) (y : @alt γ _ b) : @alt γ _ tt :=
+def add {a b} (x : alt γ a) (y : alt γ b) : alt γ tt :=
 x.to_sform + y.to_sform
 
-def mul {a b} (x : @alt γ _ a) (y : @alt γ _ b) : @alt γ _ ff :=
+def mul {a b} (x : alt γ a) (y : alt γ b) : alt γ ff :=
 x.to_pform * y.to_pform
 
-def pow {a} (x : @alt γ _ a) (n : znum) : @alt γ _ ff :=
+def pow {a} (x : alt γ a) (n : znum) : alt γ ff :=
 x.to_pform ^ n
 
-theorem hyps_singleton {b} {x : @nterm γ _} :
-  (singleton x : @alt γ _ b).hyps = ∅ :=
+theorem hyps_singleton {b} {x : nterm γ} :
+  (singleton x : alt γ b).hyps = ∅ :=
 by cases b; simp [singleton, hyps]
 
-theorem hyps_add_sform {x y : @alt γ _ tt} :
+theorem hyps_add_sform {x y : alt γ tt} :
   (x + y).hyps = x.hyps ∪ y.hyps :=
 by simp [has_add.add, add_sform, hyps]
 
-theorem hyps_mul_pform {x y : @alt γ _ ff} :
+theorem hyps_mul_pform {x y : alt γ ff} :
   (x * y).hyps = x.hyps ∪ y.hyps :=
 by simp [has_mul.mul, mul_pform, hyps]
 
-theorem hyps_pow_pform {x : @alt γ _ ff} {n : znum} :
+theorem hyps_pow_pform {x : alt γ ff} {n : znum} :
   (x ^ n).hyps = if n = 0 then ∅ else x.hyps :=
 begin
   by_cases h0 : n = 0;
@@ -167,19 +167,19 @@ begin
   simp [has_pow.pow, pow_pform, h0, h1, hyps, hyps_singleton]
 end
 
-theorem hyps_add {a b} {x : @alt γ _ a} {y : @alt γ _ b} :
+theorem hyps_add {a b} {x : alt γ a} {y : alt γ b} :
   hyps (add x y) = hyps x.to_sform ∪ hyps y.to_sform :=
 by cases x; cases y; simp [add, to_sform, hyps_add_sform]
 
-theorem hyps_mul {a b} {x : @alt γ _ a} {y : @alt γ _ b} :
+theorem hyps_mul {a b} {x : alt γ a} {y : alt γ b} :
   hyps (mul x y) = hyps x.to_pform ∪ hyps y.to_pform :=
 by cases x; cases y; simp [mul, to_pform, hyps_mul_pform]
 
-theorem hyps_pow {a} {x : @alt γ _ a} {n : znum} :
+theorem hyps_pow {a} {x : alt γ a} {n : znum} :
   hyps (pow x n) = if n = 0 then ∅ else hyps x.to_pform :=
 by simp [pow, hyps, hyps_pow_pform]
 
-theorem eval_add_sform {x y : @alt γ _ tt} :
+theorem eval_add_sform {x y : alt γ tt} :
   eval ρ (x + y) = eval ρ x + eval ρ y :=
 begin
   suffices : eval ρ (add_sform x y) = eval ρ x + eval ρ y,
@@ -189,7 +189,7 @@ begin
   apply sterm.eval_add
 end
 
-theorem eval_add {a b} {x : @alt γ _ a} {y : @alt γ _ b} :
+theorem eval_add {a b} {x : alt γ a} {y : alt γ b} :
   nonzero ρ (hyps (add x y)) →
   eval ρ (add x y) = eval ρ x + eval ρ y :=
 begin
@@ -200,7 +200,7 @@ begin
   { exact H1 }
 end
 
-theorem eval_mul_pform {x y : @alt γ _ ff} :
+theorem eval_mul_pform {x y : alt γ ff} :
   eval ρ (x * y) = eval ρ x * eval ρ y :=
 begin
   suffices : eval ρ (mul_pform x y) = eval ρ x * eval ρ y,
@@ -210,13 +210,13 @@ begin
   apply pterm.eval_mul
 end
 
-theorem eval_mul {a b} {x : @alt γ _ a} {y : @alt γ _ b} :
+theorem eval_mul {a b} {x : alt γ a} {y : alt γ b} :
   eval ρ (mul x y) = eval ρ x * eval ρ y :=
 begin
   unfold mul, rw [eval_mul_pform, eval_to_pform, eval_to_pform]
 end
 
-theorem eval_pow_pform {x : @alt γ _ ff} {n : znum} :
+theorem eval_pow_pform {x : alt γ ff} {n : znum} :
   eval ρ (x ^ n) = eval ρ x ^ (n : ℤ) :=
 begin
   suffices : eval ρ (pow_pform x n) = eval ρ x ^ (n : ℤ),
@@ -228,27 +228,27 @@ begin
   { rw if_neg hn, unfold eval, apply pterm.eval_pow }
 end
 
-theorem eval_pow {a} {x : @alt γ _ a} {n : znum} :
+theorem eval_pow {a} {x : alt γ a} {n : znum} :
   eval ρ (pow x n) = eval ρ x ^ (n : ℤ) :=
 begin
   unfold pow, rw [eval_pow_pform, eval_to_pform]
 end
 
 @[reducible]
-def aux_of_nterm : @nterm γ _ → bool
+def aux_of_nterm : nterm γ → bool
 | (nterm.add _ _) := tt
 | (nterm.mul _ _) := ff
 | (nterm.pow _ _) := ff
 | _ := tt
 
-def of_nterm : Π (x : @nterm γ _), @alt γ _ (aux_of_nterm x)
+def of_nterm : Π (x : nterm γ), alt γ (aux_of_nterm x)
 | (nterm.add x y) := add (of_nterm x) (of_nterm y)
 | (nterm.mul x y) := mul (of_nterm x) (of_nterm y)
 | (nterm.pow x n) := pow (of_nterm x) n
 | (nterm.const a) := of_const a
 | (nterm.atom i)  := singleton i
 
-theorem eval_of_nterm {x : @nterm γ _} :
+theorem eval_of_nterm {x : nterm γ} :
   nonzero ρ (of_nterm x).hyps →
   eval ρ (of_nterm x) = nterm.eval ρ x :=
 begin
@@ -288,13 +288,13 @@ variables {α : Type} [discrete_field α]
 variables {γ : Type} [const_space γ]
 variables [morph γ α] {ρ : dict α}
 
-def norm (x : @nterm γ _) : @nterm γ _ :=
+def norm (x : nterm γ) : nterm γ :=
 (alt.of_nterm x).to_sform.to_nterm
 
-def norm_hyps (x : @nterm γ _) : list (@nterm γ _) :=
+def norm_hyps (x : nterm γ) : list (nterm γ) :=
 (alt.of_nterm x).to_sform.hyps
 
-def correctness {x : @nterm γ _} :
+def correctness {x : nterm γ} :
   nonzero ρ (norm_hyps x) →
   nterm.eval ρ (norm x) = nterm.eval ρ x :=
 begin
@@ -305,7 +305,7 @@ begin
 end
 
 --section soundness
---variables {x y : @nterm γ _} {i : num} {n : znum} {c : γ}
+--variables {x y : nterm γ} {i : num} {n : znum} {c : γ}
 --
 --theorem sound_atom : @norm γ _ i = i :=
 --begin
@@ -337,13 +337,13 @@ end
 --  sorry
 --end
 --
---def naive_norm : @nterm γ _ → @nterm γ _
+--def naive_norm : nterm γ → nterm γ
 --| (add x y) := (sterm.of_nterm (naive_norm x) + sterm.of_nterm (naive_norm y)).to_nterm
 --| (mul x y) := (pterm.of_nterm (naive_norm x) * pterm.of_nterm (naive_norm y)).reduce.to_nterm
 --| (pow x n) := (pterm.of_nterm (naive_norm x) ^ n).reduce.to_nterm
 --| x := x
 --
---theorem soundness {x : @nterm γ _} :
+--theorem soundness {x : nterm γ} :
 --  norm x = naive_norm x :=
 --begin
 --  sorry
