src/tactic/field/sterm.lean
@@ -4,31 +4,30 @@ namespace field
 
 open nterm
 
-variables {α : Type} [discrete_field α]
-variables {γ : Type} [const_space γ]
-variables [morph γ α] {ρ : dict α}
-
 --@[derive decidable_eq]
-structure cterm : Type :=
-(term : @nterm γ _)
+structure cterm (γ : Type) [const_space γ] : Type :=
+(term : nterm γ)
 (coeff : γ)
 (pr : coeff ≠ 0)
 
 namespace cterm
+variables {α : Type} [discrete_field α]
+variables {γ : Type} [const_space γ]
+variables [morph γ α] {ρ : dict α}
 
-instance : inhabited (@cterm γ _) := ⟨⟨nterm.const 0, 1, by simp⟩⟩
+instance : inhabited (cterm γ) := ⟨⟨nterm.const 0, 1, by simp⟩⟩
 
-def to_nterm (x : @cterm γ _) : @nterm γ _ :=
+def to_nterm (x : cterm γ) : nterm γ :=
 if x.coeff = 0 then 0
 else if x.coeff = 1 then x.term
 else if x.term = 1 then x.coeff
 else x.term * x.coeff
 
-def eval (ρ : dict α) (x : @cterm γ _) : α :=
+def eval (ρ : dict α) (x : cterm γ) : α :=
 nterm.eval ρ x.term * ↑x.coeff
 
 @[simp]
-def eval_to_nterm {x : @cterm γ _} :
+def eval_to_nterm {x : cterm γ} :
  nterm.eval ρ x.to_nterm = cterm.eval ρ x :=
 begin
   by_cases h1 : x.coeff = 0;
@@ -38,44 +37,44 @@ begin
 end
 
 theorem eval_to_nterm' :
-  @nterm.eval _ _ γ _ _ ρ ∘ cterm.to_nterm = cterm.eval ρ :=
+  nterm.eval ρ ∘ @cterm.to_nterm γ _ = cterm.eval ρ :=
 begin
   unfold function.comp,
   simp [eval_to_nterm]
 end
 
 --TODO
-theorem eval_def {x : @nterm γ _} {c : γ} {hc : c ≠ 0} :
+theorem eval_def {x : nterm γ} {c : γ} {hc : c ≠ 0} :
   cterm.eval ρ ⟨x, c, hc⟩ = nterm.eval ρ x * ↑c :=
 rfl
 
-theorem eval_add {x : @nterm γ _} {a b : γ}
+theorem eval_add {x : nterm γ} {a b : γ}
   {ha : a ≠ 0} {hb : b ≠ 0} {hc : a + b ≠ 0} :
   cterm.eval ρ ⟨x, a + b, hc⟩ = cterm.eval ρ ⟨x, a, ha⟩ + cterm.eval ρ ⟨x, b, hb⟩ :=
 begin
   simp [eval_def, morph.morph_add, mul_add],
 end
 
-def mul (x : @cterm γ _) (a : γ) (ha : a ≠ 0) : @cterm γ _ :=
+def mul (x : cterm γ) (a : γ) (ha : a ≠ 0) : cterm γ :=
 ⟨x.term, x.coeff * a, by simp [ha, x.pr]⟩
 
-theorem eval_mul {x : @cterm γ _} {a : γ} {ha : a ≠ 0} :
+theorem eval_mul {x : cterm γ} {a : γ} {ha : a ≠ 0} :
   cterm.eval ρ (x.mul a ha) = cterm.eval ρ x * ↑a :=
 begin
   simp [cterm.eval, morph.morph_mul, mul], ring
 end
 
 theorem eval_mul' {a : γ} {ha : a ≠ 0} :
-  cterm.eval ρ ∘ (λ x : cterm, x.mul a ha) =
+  cterm.eval ρ ∘ (λ x : cterm γ, x.mul a ha) =
     λ x, cterm.eval ρ x * (a : α) :=
 begin
   unfold function.comp,
   simp [eval_mul]
 end
 
-theorem eval_sum_mul {xs : list (@cterm γ _)} {a : γ} {ha : a ≠ 0} :
+theorem eval_sum_mul {xs : list (cterm γ)} {a : γ} {ha : a ≠ 0} :
   list.sum (list.map (cterm.eval ρ) xs) * ↑a
-    = list.sum (list.map (λ x : cterm, cterm.eval ρ (x.mul a ha)) xs) :=
+    = list.sum (list.map (λ x : cterm γ, cterm.eval ρ (x.mul a ha)) xs) :=
 begin
   induction xs with x xs ih,
   { simp },
@@ -83,7 +82,7 @@ begin
     rw [eval_mul, add_mul, ih] }
 end
 
-def smerge : list (@cterm γ _) → list (@cterm γ _) → list (@cterm γ _)
+def smerge : list (cterm γ) → list (cterm γ) → list (cterm γ)
 | (x::xs) (y::ys) :=
   if x.term = y.term then
     let c := x.coeff + y.coeff in
@@ -96,7 +95,7 @@ def smerge : list (@cterm γ _) → list (@cterm γ _) → list (@cterm γ _)
 | xs [] := xs
 | [] ys := ys
 
-lemma smerge_nil_left {ys : list (@cterm γ _)} :
+lemma smerge_nil_left {ys : list (cterm γ)} :
   smerge [] ys = ys :=
 begin
   induction ys with y ys ih,
@@ -104,7 +103,7 @@ begin
   { unfold smerge }
 end
 
-lemma smerge_nil_right {xs : list (@cterm γ _)} :
+lemma smerge_nil_right {xs : list (cterm γ)} :
   smerge xs [] = xs :=
 begin
   induction xs with x xs ih,
@@ -112,24 +111,24 @@ begin
   { unfold smerge }
 end
 
-lemma smerge_def1 {x y : @cterm γ _} {xs ys : list (@cterm γ _)} :
+lemma smerge_def1 {x y : cterm γ} {xs ys : list (cterm γ)} :
   x.term = y.term → x.coeff + y.coeff = 0 →
   smerge (x::xs) (y::ys) = smerge xs ys :=
 by intros h1 h2; simp [smerge, h1, h2]
-lemma smerge_def2 {x y : @cterm γ _} {xs ys : list (@cterm γ _)} :
+lemma smerge_def2 {x y : cterm γ} {xs ys : list (cterm γ)} :
   x.term = y.term → Π (hc : x.coeff + y.coeff ≠ 0),
   smerge (x::xs) (y::ys) = ⟨x.term, x.coeff + y.coeff, hc⟩ :: smerge xs ys :=
 by intros h1 h2; simp [smerge, h1, h2]
-lemma smerge_def3 {x y : @cterm γ _} {xs ys : list (@cterm γ _)} :
+lemma smerge_def3 {x y : cterm γ} {xs ys : list (cterm γ)} :
   x.term ≠ y.term → x.term < y.term →
   smerge (x::xs) (y::ys) = x :: smerge xs (y :: ys) :=
 by intros h1 h2; simp [smerge, h1, h2]
-lemma smerge_def4 {x y : @cterm γ _} {xs ys : list (@cterm γ _)} :
+lemma smerge_def4 {x y : cterm γ} {xs ys : list (cterm γ)} :
   x.term ≠ y.term → ¬ x.term < y.term →
   smerge (x::xs) (y::ys) = y :: smerge (x::xs) ys :=
 by intros h1 h2; simp [smerge, h1, h2]
 
-theorem eval_smerge (xs ys : list (@cterm γ _)) :
+theorem eval_smerge (xs ys : list (cterm γ)) :
   list.sum (list.map (cterm.eval ρ) (smerge xs ys))
   = list.sum (list.map (cterm.eval ρ) xs)
     + list.sum (list.map (cterm.eval ρ) ys) :=
@@ -168,19 +167,23 @@ end
 
 end cterm
 
-structure sterm : Type :=
-(terms : list (@cterm γ _))
+structure sterm (γ : Type) [const_space γ] : Type :=
+(terms : list (cterm γ))
 
 namespace sterm
+variables {α : Type} [discrete_field α]
+variables {γ : Type} [const_space γ]
+variables [morph γ α] {ρ : dict α}
 
-def of_const (a : γ) : @sterm γ _ :=
+
+def of_const (a : γ) : sterm γ :=
 if ha : a = 0 then { terms := [] }
 else { terms := [⟨1, a, ha⟩] }
 
-def singleton (x : @nterm γ _) : @sterm γ _ :=
+def singleton (x : nterm γ) : sterm γ :=
 { terms := [⟨x, 1, by simp⟩] }
 
-def eval (ρ : dict α) (S : @sterm γ _) : α :=
+def eval (ρ : dict α) (S : sterm γ) : α :=
 list.sum (S.terms.map (cterm.eval ρ))
 
 theorem eval_of_const (a : γ) :
@@ -190,7 +193,7 @@ begin
   simp [of_const, sterm.eval, cterm.eval, ha]
 end
 
-theorem eval_singleton (x : @nterm γ _) :
+theorem eval_singleton (x : nterm γ) :
   sterm.eval ρ (singleton x) = nterm.eval ρ x :=
 begin
   by_cases hx : nterm.eval ρ x = 0,
@@ -198,28 +201,28 @@ begin
 end
 
 --mul
-def add (S T : @sterm γ _) : @sterm γ _ :=
+def add (S T : sterm γ) : sterm γ :=
 { terms := cterm.smerge S.terms T.terms, }
 
 --pow
-def mul (S : @sterm γ _) (a : γ) : @sterm γ _ :=
+def mul (S : sterm γ) (a : γ) : sterm γ :=
 if ha : a = 0 then { terms := [] }
 else { terms := S.terms.map (λ x, cterm.mul x a ha), }
 
-instance : has_add (@sterm γ _) := ⟨add⟩
+instance : has_add (sterm γ) := ⟨add⟩
 
-theorem add_terms {S T : @sterm γ _} :
+theorem add_terms {S T : sterm γ} :
   (S + T).terms = cterm.smerge S.terms T.terms :=
 by simp [has_add.add, add]
 
-theorem eval_add {S T : @sterm γ _} :
+theorem eval_add {S T : sterm γ} :
   sterm.eval ρ (S + T) = sterm.eval ρ S + sterm.eval ρ T :=
 begin
   unfold sterm.eval,
   rw [add_terms, cterm.eval_smerge]
 end
 
-theorem eval_mul {S : @sterm γ _} {a : γ} :
+theorem eval_mul {S : sterm γ} {a : γ} :
   sterm.eval ρ (S.mul a) = sterm.eval ρ S * ↑a :=
 begin
   by_cases ha : a = 0,
@@ -230,7 +233,7 @@ begin
      { exact ha }}
 end
 
-def to_nterm (S : @sterm γ _) : @nterm γ _ :=
+def to_nterm (S : sterm γ) : nterm γ :=
 match S.terms with
 | [] := 0
 | [x] := x.to_nterm
@@ -244,7 +247,7 @@ match S.terms with
         + x0.term ) * x0.coeff
 end
 
-theorem eval_to_nterm {S : @sterm γ _} :
+theorem eval_to_nterm {S : sterm γ} :
   sterm.eval ρ S = nterm.eval ρ S.to_nterm :=
 begin
   cases S with ts,
@@ -269,13 +272,13 @@ begin
   unfold cterm.eval, apply add_comm
 end
 
-def of_nterm : @nterm γ _ → @sterm γ _
+def of_nterm : nterm γ → sterm γ
 | (nterm.add x y) := of_nterm x + of_nterm y
 | (nterm.mul x (nterm.const a)) := (of_nterm x).mul a
 | (nterm.const a) := of_const a
 | x := singleton x
 
-theorem eval_of_nterm {x : @nterm γ _} :
+theorem eval_of_nterm {x : nterm γ} :
   sterm.eval ρ (of_nterm x) = nterm.eval ρ x :=
 begin
   induction x with i c x y ihx ihy x y ihx ihy x n ihx,
